wip

CellularAutomatas/proofs/composition.lean
@@ -1,4 +1,4 @@
---import CellularAutomatas.defs
+import CellularAutomatas.defs
 import Mathlib.Data.List.Basic
 import Mathlib.Data.Nat.Basic
 import Mathlib.Data.Nat.Find
@@ -10,183 +10,19 @@ import Mathlib.Data.Fintype.Basic
 import Mathlib.Data.Fintype.Pi
 import Mathlib.Data.Fintype.Prod
 import Mathlib.Data.Fintype.Option
+import Mathlib.Tactic.Linarith
+import CellularAutomatas.proofs.basic
+
 
 namespace CellularAutomatas
 
-notation:max t "？" => Option t
-
 notation:max x "³"  => Fin 3 → x
-
-class Alphabet (α: Type) where
-    [dec: DecidableEq α]
-    [fin: Fintype α]
-    [inh: Inhabited α]
-
-attribute [instance] Alphabet.dec Alphabet.fin Alphabet.inh
-
-instance (α: Type) [DecidableEq α] [Fintype α] [Inhabited α]: Alphabet α := {}
-
-
-def Config (Q: Type) := ℤ → Q
-def Trace (Q: Type) := ℕ → Q
-
-abbrev Word (α: Type) := List α
-
-def word_to_config {α : Type} (w : Word α) : Config (Option α) :=
-  fun p => if h : p ≥ 0 ∧ p < w.length then some w[p.toNat] else none
-
-notation "⟬" w "⟭" => word_to_config w
-
-instance : Coe (Word α) (Config α？) := ⟨word_to_config⟩
-
-
-
-structure CellAutomaton (α β: Type) where
-  Q: Type
-  [alphabetQ: Alphabet Q]
-  δ: Q → Q → Q → Q
-  embed: α → Q
-  project: Q → β
-
-attribute [instance] CellAutomaton.alphabetQ
-
-namespace CellAutomaton
-
-  def embed_config {α β: Type} {C: CellAutomaton α β} (c: Config α) : Config C.Q :=
-    fun p => C.embed (c p)
-
-  notation "⦋" w "⦌"  => embed_config w
-
-  instance {C: CellAutomaton α β} : Coe (Config α) (Config C.Q) := ⟨embed_config⟩
-
-
-  def embed_word {α β: Type} {C: CellAutomaton α？ β} (w: Word α): Config C.Q := word_to_config w
-
-  notation "⦋" w "⦌" => embed_word w
-
-  instance {C: CellAutomaton α？ β} : Coe (Word α) (Config C.Q) := ⟨embed_word⟩
-
-  @[simp]
-  lemma embed_word_word_to_config_eq {α β: Type} {C: CellAutomaton α？ β} (w: Word α):
-      C.embed_config (word_to_config w) = ⦋w⦌ := rfl
-
-  def project_config {α β: Type} (C: CellAutomaton α β) (c: Config C.Q): Config β :=
-    fun p => C.project (c p)
-
-  def next {α β: Type} (C: CellAutomaton α β) (c: Config C.Q): Config C.Q :=
-    fun p => C.δ (c (p - 1)) (c p) (c (p + 1))
-
-  def nextt {α β: Type} (C: CellAutomaton α β) (c: Config C.Q) (t: ℕ): Config C.Q :=
-    Nat.iterate (C.next) t c
-
-  def comp {α β: Type} (C: CellAutomaton α β) (c: Config C.Q): Trace (Config β) :=
-    C.project_config ∘ C.nextt c
-
-  def trace {α β: Type} (C: CellAutomaton α β) (c: Config α): Trace β := (C.comp c · 0)
-
-  def trace_rt {α β: Type} (C: CellAutomaton α？ β) (w: Word α): Word β :=
-    (List.range w.length).map (C.trace w)
-
-  def map_project {α β γ: Type} (C: CellAutomaton α β) (f: β → γ): CellAutomaton α γ :=
-    {
-      Q := C.Q
-      δ := C.δ
-      embed := C.embed
-      project := f ∘ C.project
-    }
-
-end CellAutomaton
-
-
-
-
-
-
-abbrev LCellAutomaton (α: Type) := CellAutomaton α？ Bool
-
-structure tCellAutomaton (α: Type) extends LCellAutomaton α where
-  t: ℕ → ℕ
-  p: ℕ → ℤ
-
-def tCellAutomaton.accepts {C: tCellAutomaton α} (w: Word α) := C.comp w (C.t w.length) (C.p w.length)
 
 
 open CellAutomaton
 
-@[grind =]
-lemma word_to_config_natcast_eq {w: Word α} {t: ℕ} (h: t < w.length): ⟬w⟭ ↑t = some w[t] := by simp [word_to_config, h]
 
 
-lemma trace_rt_of_map_project {α β γ: Type} {C: CellAutomaton α？ β} (f: β → γ) (w: Word α):
-      (C.map_project f).trace_rt w = (C.trace_rt w).map f := by
-  unfold trace_rt
-  apply List.ext_getElem (by simp)
-  intro i h1 h2
-  unfold trace comp project_config map_project
-  simp
-  congr 1
-
-@[simp]
-lemma trace_rt_length {α β: Type} {C: CellAutomaton α？ β} {w: Word α}:
-  (C.trace_rt w).length = w.length := by simp [trace_rt]
-
-
-
-
-
-
-section id
-
-  def ca_id (α : Type) [Alphabet α] : CellAutomaton α α := {
-    Q := α
-    δ := fun _ _ r => r
-    embed := id
-    project := id
-  }
-
-  def config_to_trace {α: Type} (c: Config α): Trace α := fun t => c t
-
-  @[simp]
-  lemma ca_id_trace_eq {α : Type} [Alphabet α]:
-    (ca_id α).trace = config_to_trace := by
-    unfold trace
-    funext t
-    conv in comp _ => change nextt _
-
-    have shift_next c : (ca_id α).next c = fun i => c (i + 1) := by
-      funext i
-      simp [CellAutomaton.next, ca_id]
-
-    have shift_nextt k c i: ((ca_id α).nextt c k) i = c (i + k) := by
-      induction k generalizing c with
-      | zero =>
-        simp [CellAutomaton.nextt, Nat.iterate]
-      | succ k ih =>
-        rw [CellAutomaton.nextt, Nat.iterate]
-        rw [shift_next]
-        rw [← CellAutomaton.nextt]
-        rw [ih]
-        grind
-    funext t
-    rw [shift_nextt]
-    conv in embed_config => change id
-    simp [config_to_trace]
-
-
-
-  def ca_id_word (α: Type) [Alphabet α] : CellAutomaton α？ α := (ca_id α？).map_project (·.getD default)
-
-  @[simp]
-  lemma ca_id_scan_temporal [Alphabet α]: (ca_id_word α).trace_rt = id := by
-    funext w
-    rw [id_eq, ca_id_word, trace_rt_of_map_project]
-    apply List.ext_getElem (by simp)
-    intro i h_i h_len
-    unfold trace_rt
-    simp [ca_id_trace_eq]
-    grind [ca_id_trace_eq, config_to_trace]
-
-end id
 
 
 
@@ -265,10 +101,63 @@ namespace CompressToΛ
 
 end CompressToΛ
 
-lemma intCastEq {k: ℕ} [NeZero k] (p: ℤ): (Fin.intCast p: Fin k) = (p % k) := by
-  sorry
+lemma intCastEq {k: ℕ} [NeZero k] (p: ℤ): ((Fin.intCast p: Fin k) : ℤ) = p % k := by
+  unfold Fin.intCast
+  split_ifs with h
+  · lift p to ℕ using h
+    simp
+  · push_neg at h
+    rw [Fin.val_neg]
+    simp only [Fin.val_ofNat]
+    have hp : p = -↑(p.natAbs) := by
+      rw [←neg_neg p, ←Int.ofNat_natAbs_of_nonpos (le_of_lt h)]
+      simp
+    rw [hp]
+    rw [Int.neg_emod]
+    simp only [Int.natAbs_neg, Int.natAbs_natCast]
+    by_cases hk : k ∣ p.natAbs
+    · simp only [Fin.ofNat_eq_cast, Fin.natCast_eq_zero, hk, ↓reduceIte, Nat.cast_zero,
+      Int.ofNat_dvd.mpr hk]
+    · have h_not_dvd : ¬ (↑k : ℤ) ∣ ↑p.natAbs := mt Int.ofNat_dvd.mp hk
+      simp only [Fin.ofNat_eq_cast, Fin.natCast_eq_zero, hk, ↓reduceIte, h_not_dvd]
+      rw [Int.ofNat_sub]
+      · simp only [Int.natCast_emod]
+      · apply le_of_lt
+        apply Nat.mod_lt
+        exact NeZero.pos k
+
+lemma nextt_shift {α β: Type} (C: CellAutomaton α β) (c: Config C.Q) (t: ℕ) (x d: ℤ):
+    C.nextt c t (x + d) = C.nextt (fun i => c (i + d)) t x := by
+  induction t generalizing x with
+  | zero => simp
+  | succ t ih =>
+    rw [nextt_succ, nextt_succ]
+    unfold CellAutomaton.next
+    have h1 : x + d - 1 = x - 1 + d := by ring
+    have h2 : x + d + 1 = x + 1 + d := by ring
+    rw [h1, h2]
+    rw [ih (x-1), ih x, ih (x+1)]
+
+lemma nextt_locality {α β: Type} (C: CellAutomaton α β) (c1 c2: Config C.Q) (t: ℕ) (x: ℤ):
+    (∀ y, x - t ≤ y ∧ y ≤ x + t → c1 y = c2 y) → C.nextt c1 t x = C.nextt c2 t x := by
+  induction t generalizing x with
+  | zero =>
+    intro h
+    apply h
+    simp
+  | succ t ih =>
+    intro h
+    rw [nextt_succ, nextt_succ]
+    unfold CellAutomaton.next
+    grind
 
 
+
+lemma nextt_add {α β: Type} (C: CellAutomaton α β) (c: Config C.Q) (t1 t2: ℕ):
+    C.nextt c (t1 + t2) = C.nextt (C.nextt c t1) t2 := by
+  rw [Nat.add_comm]
+  rw [nextt, Function.iterate_add_apply]
+  rfl
 
 structure SpeedupKx where
   k: ℕ
@@ -327,12 +216,84 @@ namespace SpeedupKx
 
 
   lemma compression_k_step (c: Config e.C_orig.Q):
-      e.C.next (compress e.k c) = compress e.k (e.C_orig.nextt c e.k) :=
-        sorry
+      e.C.next (compress e.k c) = compress e.k (e.C_orig.nextt c e.k) := by
+    funext p j
+    simp [CellAutomaton.next, C, compress, to_local_config]
+    rw [add_comm (p * e.k) j]
+    rw [nextt_shift]
+    apply nextt_locality
+    intro y hy
+    have hk : (e.k : ℤ) ≥ 1 := by
+      have : e.k ≠ 0 := NeZero.ne e.k
+      omega
+    have hj : 0 ≤ (j : ℤ) ∧ (j : ℤ) < e.k := by
+      constructor
+      · simp
+      · simp
+    unfold local_config
+    split_ifs with h1 h2 h3
+    · -- y <= -k
+      have : y = -e.k := by omega
+      subst y
+      unfold compress
+      rw [intCastEq]
+      simp
+      apply congrArg
+      ring
+    · -- -k < y < 0
+      unfold compress
+      rw [intCastEq]
+      have h_pos : 0 ≤ y + ↑e.k := by omega
+      have h_lt : y + ↑e.k < ↑e.k := by omega
+      rw [Int.emod_eq_of_lt h_pos h_lt]
+      apply congrArg
+      ring
+    · -- 0 <= y < k
+      unfold compress
+      rw [intCastEq]
+      have h_pos : 0 ≤ y := by omega
+      have h_lt : y < ↑e.k := by omega
+      rw [Int.emod_eq_of_lt h_pos h_lt]
+      apply congrArg
+      ring
+    · -- k <= y
+      unfold compress
+      rw [intCastEq]
+      have h_pos : 0 ≤ y - ↑e.k := by omega
+      have h_lt : y - ↑e.k < ↑e.k := by omega
+      rw [Int.emod_eq_of_lt h_pos h_lt]
+      apply congrArg
+      ring
 
   theorem spec {c: Config e.α}:
-      ∀ t, e.C.comp ⦋(compress e.k c)⦌ t = compress e.k (e.C_orig.comp c (e.k * t)) :=
-        sorry
+      ∀ t, e.C.comp ⦋(compress e.k c)⦌ t = compress e.k (e.C_orig.comp c (e.k * t)) := by
+    intro t
+    unfold CellAutomaton.comp CellAutomaton.project_config
+    funext p
+    let c_orig : Config e.C_orig.Q := ⦋c⦌
+    have h_comm : (⦋compress e.k c⦌: Config e.C.Q) = compress e.k c_orig := by
+      funext p j
+      simp [compress, CellAutomaton.embed_config, C]
+      rfl
+    dsimp [CellAutomaton.embed_config] at h_comm ⊢
+    change e.C.project ((e.C.nextt (e.C.embed_config (compress e.k c)) t) p) = _
+    have h_eq : e.C.nextt ⦋compress e.k c⦌ t = e.C.nextt (compress e.k c_orig) t := by
+      congr 1
+    rw [h_eq]
+    have h_state : e.C.nextt (compress e.k c_orig) t = compress e.k (e.C_orig.nextt c_orig (e.k * t)) := by
+      induction t with
+      | zero => simp
+      | succ t ih =>
+        rw [CellAutomaton.nextt_succ]
+        rw [ih]
+        rw [compression_k_step]
+        rw [mul_add, mul_one]
+        rw [nextt_add]
+        grind
+    rw [h_state]
+    unfold compress
+    simp [C]
+    rfl
 
   theorem spec1 {c: Config e.α} {t1: ℕ}:
       e.C.trace (compress e.k c) t1 0 = e.C_orig.trace c (e.k * t1) := by
@@ -356,14 +317,75 @@ namespace TraceKx
 
   variable (e: TraceKx)
 
-  -- cell at (t + k,p) has state of orig at (t + {0,1,...,k-1}, p)
-  def C: CellAutomaton e.α (Fin e.k → e.β？) := sorry
+  def C: CellAutomaton e.α (Fin e.k → e.β？) := {
+    Q := Fin (e.k + 1) → e.C_orig.Q
+    δ := fun a b c =>
+      let next_s := e.C_orig.δ (a (Fin.last e.k)) (b (Fin.last e.k)) (c (Fin.last e.k))
+      Fin.snoc (Fin.tail b) next_s
+    embed := fun a =>
+      let s := e.C_orig.embed a
+      fun _ => s
+    project := fun q =>
+      fun i => some (e.C_orig.project (q (i.castSucc)))
+  }
+
+  lemma state_eq (c: Config e.α) (t: ℕ) (p: ℤ) (i: Fin (e.k + 1)):
+      (e.C.nextt ⦋c⦌ t p) i = (e.C_orig.nextt ⦋c⦌ (t + i - e.k) p) := by
+    revert p i
+    induction t with
+    | zero =>
+      intros p i
+      simp [C, CellAutomaton.embed_config]
+      have : (i : ℕ) - e.k = 0 := Nat.sub_eq_zero_of_le (Nat.le_of_lt_succ i.isLt)
+      rw [this]
+      rw [nextt_zero]
+      rfl
+    | succ t ih =>
+      intros p i
+      rw [CellAutomaton.nextt_succ]
+      unfold CellAutomaton.next C
+      simp
+      by_cases h: i = Fin.last e.k
+      · rw [h]
+        simp [Fin.snoc]
+        change e.C_orig.δ (e.C.nextt ⦋c⦌ t (p - 1) (Fin.last e.k)) (e.C.nextt ⦋c⦌ t p (Fin.last e.k)) (e.C.nextt ⦋c⦌ t (p + 1) (Fin.last e.k)) = _
+        rw [ih (p-1) (Fin.last e.k), ih p (Fin.last e.k), ih (p+1) (Fin.last e.k)]
+        simp [CellAutomaton.next]
+      · have h_lt : (i : ℕ) < e.k := by
+          apply Nat.lt_of_le_of_ne
+          · apply Nat.le_of_lt_succ
+            exact i.isLt
+          · intro heq
+            apply h
+            ext
+            simp [heq]
+        have h_cast : i = Fin.castSucc ⟨i, h_lt⟩ := by
+          ext
+          simp
+        rw [h_cast]
+        simp [Fin.snoc, h_lt]
+        change e.C.nextt ⦋c⦌ t p (Fin.succ ⟨i, h_lt⟩) = _
+        rw [ih p (Fin.succ ⟨i, h_lt⟩)]
+        congr 1
+        simp
+        rw [Nat.add_comm (↑i) 1]
+        rw [←Nat.add_assoc]
 
   theorem spec (c: Config e.α) (t1: ℕ) (p: ℤ):
       e.C.comp c (t1 + e.k) p =
         fun (t2: Fin e.k) => some (e.C_orig.comp c (t1 + t2) p)
       := by
-    sorry
+    unfold CellAutomaton.comp CellAutomaton.project_config
+    simp only [C]
+    simp
+    change (fun (t2 : Fin e.k) => some (e.C_orig.project ((e.C.nextt ⦋c⦌ (t1 + e.k) p) t2.castSucc))) = _
+    funext t2
+    rw [state_eq]
+    congr
+    simp
+    rw [Nat.add_right_comm]
+    rw [Nat.add_sub_cancel]
+
 end TraceKx
 
 structure SpeedupAndTraceKx where
@@ -404,9 +426,24 @@ namespace SpeedupAndTraceKx
 
   theorem spec1 {c: Config e.α} {t1: ℕ} {t2: Fin e.k}:
       e.C.trace (SpeedupKx.compress e.k c) (t1 + 1) t2 = e.C_orig.trace c (e.k * t1 + t2) := by
-        unfold trace
-        -- should be trivial
-        sorry
+    unfold trace
+    have h_comp : ∀ t p, e.C.comp ⦋SpeedupKx.compress e.k c⦌ t p = (fun g i => (g 0 i).getD default) (e.SP.C.comp ⦋SpeedupKx.compress e.k c⦌ t p) := by
+      intros t p
+      unfold CellAutomaton.comp CellAutomaton.project_config
+      simp [C]
+      rfl
+    rw [h_comp]
+    have h_spec : e.SP.C.comp ⦋SpeedupKx.compress e.k c⦌ (t1 + 1) = SpeedupKx.compress e.k (e.T.C.comp c (e.k * (t1 + 1))) := by
+      convert e.SP.spec (t1 + 1)
+    rw [h_spec]
+    unfold SpeedupKx.compress
+    simp only
+    rw [mul_add, mul_one]
+    have h_spec_T : e.T.C.comp c (e.k * t1 + e.k) 0 = fun (t2 : Fin e.k) => some (e.C_orig.comp c (e.k * t1 + t2) 0) := by
+      convert e.T.spec c (e.k * t1) 0
+    simp only [zero_mul, zero_add]
+    erw [h_spec_T]
+    simp
 
 
 end SpeedupAndTraceKx
@@ -429,31 +466,51 @@ attribute [instance] SimFromΛ._inst_γ
 namespace SimFromΛ
   variable (e: SimFromΛ)
 
-  structure Q1 where
+  structure Q where
     state: e.C_ctl.Q
     counter: Fin 3
+    sim: Option (e.C_inr.Q × e.C_inr.Q)
   deriving Inhabited, DecidableEq
 
   -- TODO@hediet - why cannot I derive Fintype automatically here?
-  instance : Fintype (Q1 e) :=
-    Fintype.ofEquiv (e.C_ctl.Q × Fin 3)
-    { toFun := fun x => ⟨x.1, x.2⟩
-      invFun := fun x => (x.1, x.2)
+  instance : Fintype (Q e) :=
+    Fintype.ofEquiv (e.C_ctl.Q × Fin 3 × Option (e.C_inr.Q × e.C_inr.Q))
+    { toFun := fun x => ⟨x.1, x.2.1, x.2.2⟩
+      invFun := fun x => (x.state, x.counter, x.sim)
       left_inv := fun _ => rfl
       right_inv := fun _ => rfl }
 
+  def get_neighbor_val (q: Q e) : e.C_inr.Q :=
+    match q.sim with
+    | some (new, old) => if q.counter == 1 then old else new
+    | none => default
 
   def C: CellAutomaton e.α e.γ？ := {
-    Q := Option (Q1 e × e.C_inr.Q)
-    δ := fun a b c =>
-      match (a, b, c) with
-      | (some qa, some (qb, _), some qc) =>
-        if qb.counter = 2
-        then sorry
-        else none
-      | _ => none
-    embed := sorry
-    project := sorry
+    Q := Q e
+    δ := fun qa qb qc =>
+        let next_q_ctl := e.C_ctl.δ qa.state qb.state qc.state
+        let trigger := e.C_ctl.project next_q_ctl
+        match trigger with
+        | some s =>
+          { state := next_q_ctl, counter := 0, sim := some (e.C_inr.embed s, e.C_inr.embed s) }
+        | none =>
+          match qb.sim with
+          | some (new_b, old_b) =>
+             if qb.counter == 2 then
+               let val_a := e.get_neighbor_val qa
+               let val_c := e.get_neighbor_val qc
+               let next_val := e.C_inr.δ val_a new_b val_c
+               { state := next_q_ctl, counter := 0, sim := some (next_val, new_b) }
+             else
+               { state := next_q_ctl, counter := qb.counter + 1, sim := some (new_b, old_b) }
+          | none =>
+             { state := next_q_ctl, counter := 0, sim := none }
+    embed := fun a =>
+      { state := e.C_ctl.embed a, counter := 0, sim := none }
+    project := fun q =>
+      match q.sim with
+      | some (new, _) => some (e.C_inr.project new)
+      | none => none
   }
 
   variable (c_ctl: Config e.α)
@@ -467,9 +524,27 @@ namespace SimFromΛ
       else none
 
 
+  lemma state_track (t: ℕ) (p: ℤ):
+    (e.C.nextt ⦋c_ctl⦌ t p).state = e.C_ctl.nextt ⦋c_ctl⦌ t p := by
+    induction t generalizing p with
+    | zero =>
+      simp [CellAutomaton.embed_config, C]
+    | succ t ih =>
+      rw [CellAutomaton.nextt_succ, CellAutomaton.nextt_succ]
+      simp [CellAutomaton.next, C]
+      sorry
+
+  def T (t: ℕ) (p: ℤ) (k: ℕ) := 3 * t + 3 + 2 * p.natAbs + k
+
+  lemma T_reset_iff (t: ℕ) (p: ℤ) (k: Fin 3):
+    T t p k = 3 + 2 * p.natAbs ↔ t = 0 ∧ k = 0 := by
+    unfold T
+    omega
+
   theorem spec (h_CM: e.c_ctl_computes_c_inr c_ctl c_inr) (t: ℕ):
     e.C.trace c_ctl (3 * t + 3) = some (e.C_inr.trace c_inr t) := by
-      sorry
+    sorry
+
 end SimFromΛ
 
 
@@ -552,10 +627,13 @@ namespace AddBorder
 
   def C: CellAutomaton e.α？ e.β？ := {
     Q := e.C_orig.Q？
-    δ := fun
-    | _, _, none => none
-    | a, b, c => some (e.C_orig.δ (a.getD e.b) (b.getD e.b) (c.getD e.b))
-    embed a := Option.map e.C_orig.embed (some a)
+    δ := fun a b c =>
+      match b, c with
+      | some vb, some vc => some (e.C_orig.δ (a.getD e.b) vb vc)
+      | _, _ => none
+    embed := fun
+      | some a => some (e.C_orig.embed (some a))
+      | none => none
     project := Option.map e.C_orig.project
   }
 
@@ -670,3 +748,22 @@ namespace Composition
 
 
 end Composition
+
+def CArtTransducer.compose {α β γ} [Alphabet α] [Alphabet β] [Alphabet γ]
+    (C2: CArtTransducer β γ) (C1: CArtTransducer α β): CArtTransducer α γ :=
+  ({ α := α, β := β, γ := γ, C2 := C2, C1 := C1 }: Composition).C
+
+infixr:90 "⊚"  => CArtTransducer.compose
+
+@[simp]
+theorem CArtTransducer.compose_spec {α β γ} [Alphabet α] [Alphabet β] [Alphabet γ]
+    (C2: CArtTransducer β γ) (C1: CArtTransducer α β):
+    (C2.compose C1).trace_rt = C2.trace_rt ∘ C1.trace_rt := by
+  simp [compose]
+  rw [Composition.spec]
+
+@[simp]
+theorem CArtTransducer.compose_spec2 {α β γ} [Alphabet α] [Alphabet β] [Alphabet γ]
+    (C2: CArtTransducer β γ) (C1: CArtTransducer α β):
+    (C2.compose C1).advice.f = C2.advice.f ∘ C1.advice.f := by
+  simp [CArtTransducer.advice]
