CellularAutomatas_old/proofs/advice_two_stage_closed_under_composition.lean
@@ -9,17 +9,41 @@ import Mathlib.Data.Fintype.Prod
 import Mathlib.Data.Fintype.Option
 import Mathlib.Data.Option.Basic
 import CellularAutomatas.defs
+import CellularAutomatas.proofs.advice_prefixes_in_L_rt_closed
+import CellularAutomatas.proofs.is_two_stage_of_rt_closed_and_prefix_stable
+import CellularAutomatas.proofs.cart_transducers
 import CellularAutomatas.proofs.finite_state_transducers
+import CellularAutomatas.proofs.lcellautomaton
 import Mathlib.Tactic
-import CellularAutomatas.proofs.composition
-import CellularAutomatas.proofs.basic
 
 namespace CellularAutomatas
 
 open FiniteStateTransducer (M_map M_prod M_projQ M_id)
 
+section
+
+  variable {α β: Type} (w: Word (α × β))
+
+  def Word.fst: Word α := w.map Prod.fst
+  def Word.snd: Word β := w.map Prod.snd
+
+  @[simp] lemma Word.fst_len: (w.fst).length = w.length := by simp [Word.fst]
+  @[simp] lemma Word.snd_len: (w.snd).length = w.length := by simp [Word.snd]
+
+  @[simp] lemma Word.get_fst (t: Fin w.length): (w.fst)[t] = w[t].1 := by simp [Word.fst]
+  @[simp] lemma Word.get_snd (t: Fin w.length): (w.snd)[t] = w[t].2 := by simp [Word.snd]
+
+  @[simp] lemma Word.get_fst_ (t: ℕ) (h: t < (w.fst).length): (w.fst)[t]'h = ((w[t]'(by simp_all)).1) := by simp [Word.fst]
+  @[simp] lemma Word.get_snd_ (t: ℕ) (h: t < (w.snd).length): (w.snd)[t]'h = ((w[t]'(by simp_all)).2) := by simp [Word.snd]
+end
+
+
+@[simp] lemma LCellAutomaton.scan_temporal_rt_len {C: LCellAutomaton α} {w: Word α}:
+    (C.scan_temporal_rt w).length = w.length := by
+  simp [LCellAutomaton.scan_temporal_rt, LCellAutomaton.scan_temporal, List.length_map]
 
 namespace backwards_fsm
+
 
 
   structure Params where
@@ -46,54 +70,79 @@ namespace backwards_fsm
         let q_center := e.M.δ? q_right al
         e.C.δ (fl q_center) (fc q_right) (fr q)
       )
-    embed := fun
-    | some a => (some a, fun q => e.C.embed (e.M.f q))
-    | none => (none, fun _ => e.C.embed none)
-    project := fun (a, f) => (a.getD default, f)
+    border := (none, fun _ => e.C.border)
+    embed := fun a => (some a, fun q => e.C.embed (e.M.f q))
+    f := fun (a, f) => (a.getD default, f)
   }
 
   def M_join [Alphabet γ] [Alphabet α] [Alphabet β] (M: FiniteStateTransducer α β): FiniteStateTransducer (α × (β → γ)) γ :=
-    (M_map (fun (a, b) => a b)) ⊚ ((M_map Prod.snd) ⨂₂ (M ⊚ M_map Prod.fst))
-
+    (M_map (fun (a, b) => a b)) ⊚ (M_prod
+      (M_map Prod.snd)
+      (M ⊚ M_map Prod.fst)
+    )
 
   lemma M_join_spec (γ) [Alphabet α] [Alphabet β] [Alphabet γ] (M: FiniteStateTransducer α β) (w: Word (α × (β → γ))):
     (M_join M).scanr w = List.zipWith (· ·) w.snd (M.scanr w.fst) := by
     simp [M_join, List.zip_eq_zipWith, Word.fst, Word.snd]
 
 
-  def M' := M_map e.C.project ⊚ (M_join (M_projQ e.M))
+  def M' := M_map e.C.f ⊚ (M_join (M_projQ e.M))
+
 
 
   lemma scanr_get'_eq2 {M: FiniteStateTransducer α β} (w: Word α) (i: ℤ) (h: i ∈ w.range):
     (M.scanr w).get' i (by simp [h]) = M.f (M.scanr_reduce w⟦(i).toNat..*⟧) := by
     rw [Word.get']
     have x := M.scanr_get'_eq2 w ⟨ i.toNat, by simp_all [Word.range] ⟩
-    rw [←x]
-    congr
-
+    simp at x
+    simp [←x]
 
 
 
   lemma inv (w: Word e.α) (t: ℕ) (p: ℤ):
-      let c' := (C' e).nextt w t p
+      let c' := (C' e).comp w t p
       let q := e.M.scanr_reduce w⟦(p+t).toNat..*⟧
-      c'.2 q = (e.C.nextt (e.M.scanr w) t p)
+      c'.2 q = (e.C.comp (e.M.scanr w) t p)
       ∧ c'.1 = w.get'? (p + t) := by
-
     induction t generalizing p with
     | zero =>
-      by_cases h : p ∈ w.range
-      <;> simp [h, C', Word.get'?, scanr_get'_eq2]
+      rw [LCellAutomaton.comp_zero]
+      rw [LCellAutomaton.comp_zero]
+
+
+      set c' := (C' e).embed_word w p with h_c'
+      set c := e.C.embed_word (e.M.scanr w) p with h_c
+      set q := e.M.scanr_reduce w⟦(p + (0: ℕ)).toNat..*⟧ with h_q
+
+      constructor
+
+      case zero.right =>
+        unfold Word.get'?
+        rw [h_c']
+        simp [C', LCellAutomaton.embed_word]
+        grind
+
+      rw [h_c']
+      rw [h_c]
+      simp [C', LCellAutomaton.embed_word]
+
+      by_cases h: p ∈ w.range
+      case neg => simp [h]
+      case pos =>
+        simp [h]
+        rw [scanr_get'_eq2]
+        grind
+        simp [h]
+
+
 
     | succ t ih =>
 
-
-      set c' := (C' e).nextt w (t + 1) p with h_c'
+      set c' := (C' e).comp w (t + 1) p with h_c'
       set q := e.M.scanr_reduce w⟦(p + ↑(t+1)).toNat..*⟧ with h_q
 
-      rw [CellAutomaton.nextt_succ] at h_c'
-
-      set c'_t := ((C' e).nextt w t) with h_c'_t
+      rw [LCellAutomaton.comp_succ_eq] at h_c'
+      set c'_t := ((C' e).comp w t) with h_c'_t
 
       unfold CellAutomaton.next at h_c'
 
@@ -120,7 +169,7 @@ namespace backwards_fsm
 
       have ih_p1 := ih (p + 1)
 
-      have h1 : qr.2 q1 = e.C.nextt (e.M.scanr w) t (p + 1) ∧ qr.1 = (w.get'? (p + ↑t + 1)) := by
+      have h1 : qr.2 q1 = e.C.comp (e.M.scanr w) t (p + 1) ∧ qr.1 = (w.get'? (p + ↑t + 1)) := by
         have q_eq : e.M.scanr_reduce w⟦(p + 1 + ↑t).toNat..*⟧ = q := by
           have : (p + 1 + ↑t).toNat = (p + (↑t + 1)).toNat := by omega
           simp [this, q]
@@ -142,7 +191,7 @@ namespace backwards_fsm
         simp [h2_1]
         grind
 
-      have h2 : (qc.2 q2) = e.C.nextt (e.M.scanr w) t p := by
+      have h2 : (qc.2 q2) = e.C.comp (e.M.scanr w) t p := by
         have ih_0 := ih p
         simp [ih_0, q2_eq, qc]
 
@@ -151,26 +200,27 @@ namespace backwards_fsm
         have ih_m1 := ih (p - 1)
         grind
 
-      have q3_eq : q3 = e.M.scanr_reduce w⟦(p - 1 + ↑t).toNat..*⟧ := by
+      have h3 : (ql.2 q3) = e.C.comp (e.M.scanr w) t (p - 1) := by
+        have ih_m1 := ih (p - 1)
+
+        have q3_eq : q3 = e.M.scanr_reduce w⟦(p - 1 + ↑t).toNat..*⟧ := by
           simp [q3, q2_eq]
           conv =>
             rhs
             rw [FiniteStateTransducer.scanr_reduce'?]
           grind
-
-      have h3 : (ql.2 q3) = e.C.nextt (e.M.scanr w) t (p - 1) := by
-        have ih_m1 := ih (p - 1)
         simp [h_ql, ih_m1, q3_eq]
 
       constructor
-      · simp [h1.1, h2, h3, CellAutomaton.next]
-      · dsimp
-        change (c'_t (p+1)).1 = _
-        rw [← h_qr]
-        rw [h1.2]
-        congr 1
-        omega
+      simp [h1.1, h2, h3, q3, LCellAutomaton.comp_succ_eq, CellAutomaton.next]
+      grind
 
+  @[simp]
+  lemma Word.get'_eq (w: Word α) (i: ℕ) (h: i < w.length) (val: α): (w.get'? ↑i).getD val = w[i] := by
+    simp [Word.get'?]
+    by_cases h: ↑↑i ∈ w.range
+    simp [h, Word.get']
+    simp_all [Word.range]
 
 
   lemma spec_: (M' e).advice.f ∘ (C' e).advice.f = e.C.advice.f ∘ e.M.advice.f := by
@@ -178,48 +228,48 @@ namespace backwards_fsm
 
       unfold FiniteStateTransducer.advice
       simp [CArtTransducer.advice, M']
+      congr
+      rw [M_join_spec]
+      set c' := (C' e).scan_temporal_rt w with eq_c'
 
-      simp [backwards_fsm.M_join_spec e.C.Q]
+      have : Word.fst (List.map (C' e).f c') = w := by
+        apply List.ext_getElem
+        · simp [c']
+        intro i h1 h2
+        have inv := (inv e w i 0).2
+        simp
+        simp [LCellAutomaton.scan_temporal_rt, LCellAutomaton.scan_temporal] at eq_c'
+        simp [eq_c']
+        conv =>
+          pattern (C' e).f
+          simp [C']
+        simp [inv]
+        rw [Word.get'_eq]
 
+      rw [this]
 
-      set c' := (C' e).trace_rt w with eq_c'
+      have : Word.snd (List.map (C' e).f c') = c'.snd := by
+        unfold C'
+        simp [Word.snd]
+
+      rw [this]
 
       apply List.ext_getElem
-      · simp_all
+      · simp [eq_c']
+        rw [LCellAutomaton.scan_temporal_rt_len]
 
 
       intro i h1 h2
+
       simp
 
-      have h_w : Word.fst c' = w := by
-        apply List.ext_getElem
-        · simp_all
-        intro t ht1 ht2
-        simp [eq_c']
-
-        simp [CellAutomaton.trace_rt, CellAutomaton.trace, comp_eq_project_nextt]
-
-        have x := (inv e w t 0).2
-        conv in (CellAutomaton.project (C' e)) =>
-          simp [C']
-        simp [x]
-        rw [Word.get'_eq]
-
-      simp [h_w]
-      simp [eq_c']
-      simp [CellAutomaton.trace_rt, CellAutomaton.trace, comp_eq_project_nextt]
-
-      congr
-
-
-      have x := inv e w i 0
+      have x := (inv e w i 0).1
       simp at x
-      conv in (CellAutomaton.project (C' e)) =>
-        simp [C']
-      simp
-      rw [x.1]
 
+      simp [eq_c']
 
+      unfold LCellAutomaton.scan_temporal_rt LCellAutomaton.scan_temporal
+      simp [x]
 
 
   theorem spec {α β γ: Type} [Alphabet α] [Alphabet β] [Alphabet γ]
@@ -240,12 +290,12 @@ lemma TwoStageAdvice.from_transducers_eq {β: Type} [Alphabet α] [Alphabet β] 
     (TwoStageAdvice.from_transducers M C).advice.f = M.advice.f ∘ C.advice.f := by rfl
 
 
-def compose_two_stage [Alphabet α] [Alphabet Γ1] [Alphabet Γ] (a2: TwoStageAdvice Γ1 Γ) (a1: TwoStageAdvice α Γ1):
+def compose_two_stage [Alphabet α] [Alphabet Γ1] [Alphabet Γ] (a1: TwoStageAdvice α Γ1) (a2: TwoStageAdvice Γ1 Γ):
     TwoStageAdvice α Γ :=
   let e := backwards_fsm.Params.mk a1.M a2.C
   let ca_new := (backwards_fsm.C' e).compose a1.C
-  let fst_new := a2.M ⊚ backwards_fsm.M' e
-  TwoStageAdvice.from_transducers fst_new ca_new
+  let fsm_new := a2.M ⊚ backwards_fsm.M' e
+  TwoStageAdvice.from_transducers fsm_new ca_new
 
 
 
@@ -253,15 +303,15 @@ variable [Alphabet Γ'] [Alphabet Γ] [Alphabet α]
 
 lemma TwoStageAdvice.advice_eq (t: TwoStageAdvice α Γ):
     t.advice.f = (t.M.advice.f) ∘ (t.C.advice.f) := by
-    simp [TwoStageAdvice.advice, FiniteStateTransducer.advice, CArtTransducer.advice]
+    simp [TwoStageAdvice.advice]
 
 theorem advice_two_stage_closed_under_composition (a1: TwoStageAdvice α Γ') (a2: TwoStageAdvice Γ' Γ):
-    (compose_two_stage a2 a1).advice.f = a2.advice.f ∘ a1.advice.f := by
+    (compose_two_stage a1 a2).advice.f = a2.advice.f ∘ a1.advice.f := by
 
   rw [Eq.comm]
 
   let e := backwards_fsm.Params.mk a1.M a2.C
-  let ca_new := (backwards_fsm.C' e) ⊚ a1.C
+  let ca_new := (backwards_fsm.C' e).compose a1.C
   let fsm_new := a2.M ⊚ backwards_fsm.M' e
 
   calc (a2.advice.f ∘ a1.advice.f)
@@ -278,11 +328,8 @@ theorem advice_two_stage_closed_under_composition (a1: TwoStageAdvice α Γ') (a
       simp [Function.comp_assoc]
 
     _ = fsm_new.advice.f ∘ ca_new.advice.f := by
-      rw [CArtTransducer.compose_spec2]
+      rw [CArtTransducer.compose_spec]
       rw [FiniteStateTransducer.compose_spec]
 
     _ = (TwoStageAdvice.from_transducers fsm_new ca_new).advice.f := by simp [TwoStageAdvice.from_transducers_eq]
-    _ = (compose_two_stage a2 a1).advice.f := by rfl
-
-
-infixr:90 "⊚"  => compose_two_stage
+    _ = (compose_two_stage a1 a2).advice.f := by rfl
