CellularAutomatas_old/open_questions.lean
@@ -7,7 +7,14 @@ import Mathlib.Data.Set.Lattice
 import Mathlib.Data.Nat.Lattice
 import Mathlib.Data.Fintype.Prod
 import CellularAutomatas.defs
-import CellularAutomatas.proofs.finite_state_transducers
-import CellularAutomatas.proofs.basic
 
 namespace CellularAutomatas
+variable {α: Type} [Alphabet α]
+variable {Γ: Type} [Alphabet Γ]
+
+-- open question: is every rt_closed advice a two-stage advice?
+theorem open_question_1 (adv: Advice α Γ) (h: adv.rt_closed): adv.is_two_stage_advice := by
+    sorry
+
+theorem lt_eq_rt: CA_rt α = CA_lt α := by
+    sorry
