CellularAutomatas_old/results.lean
@@ -1,0 +1,33 @@
+import Mathlib.Data.Set.Basic
+import Mathlib.Data.Nat.Basic
+import Mathlib.Data.Nat.Find
+import Mathlib.Data.Fintype.Basic
+import Mathlib.Computability.Language
+import Mathlib.Data.Set.Lattice
+import Mathlib.Data.Nat.Lattice
+import Mathlib.Data.Fintype.Prod
+import CellularAutomatas.defs
+import CellularAutomatas.proofs.middle_not_two_stage
+import CellularAutomatas.proofs.advice_prefixes_in_L_rt_closed
+import CellularAutomatas.proofs.is_two_stage_of_rt_closed_and_prefix_stable
+
+open CellularAutomatas
+
+namespace CellularAutomatas.results
+
+variable {α} [Alphabet α]
+variable {Γ} [Alphabet Γ]
+
+theorem result_middle_not_two_stage_advice:
+    ¬ Advice.is_two_stage_advice (Advice.middle α) := by
+  exact middle_not_two_stage_advice
+
+theorem result_advice_prefixes_in_L_is_two_stage_advice:
+    ∀ C ∈ CA_rt α, Advice.is_two_stage_advice (Advice.prefixes_in_L C.L) := by
+  intro C h
+  exact advice_prefixes_in_L_is_two_stage_advice ⟨ C, h ⟩
+
+theorem result_is_two_stage_of_rt_closed_and_prefix_stable:
+    ∀ adv: Advice α Γ, adv.rt_closed ∧ adv.prefix_stable → adv.is_two_stage_advice := by
+  intro adv h
+  exact is_two_stage_of_rt_closed_and_prefix_stable adv h.1 h.2
